code/bignum/Hacl.Bignum.Fproduct.fst
@@ -20,13 +20,12 @@ val copy_from_wide_:
   output:felem ->
   input:felem_wide{disjoint output input} ->
   Stack unit
-    (requires (fun h -> live h output /\ live h input /\ copy_from_wide_pre (as_seq h input)
-      /\ (forall (i:nat). (i < len) ==> v (get h output i) == w (get h input i))))
+    (requires (fun h -> live h output /\ live h input /\ copy_from_wide_pre (as_seq h input)))
     (ensures (fun h0 _ h1 -> live h0 input /\ copy_from_wide_pre (as_seq h0 input) /\ live h1 output
       /\ modifies_1 output h0 h1
       /\ as_seq h1 output == copy_from_wide_spec (as_seq h0 input) ))
 [@"c_inline"]
-let rec copy_from_wide_ output input  =
+let copy_from_wide_ output input  =
   C.Loops.map output input clen (fun x -> wide_to_limb x)
 
 
@@ -137,7 +136,7 @@ val carry_wide_:
       /\ carry_wide_pre (as_seq h0 t) 0
       /\ as_seq h1 t == carry_wide_spec (as_seq h0 t)))
 [@"c_inline"]
-let rec carry_wide_ tmp =
+let carry_wide_ tmp =
   let h0 = ST.get() in
   let inv (h1: HyperStack.mem) (j: nat): Type0 =
     live h1 tmp /\ modifies_1 tmp h0 h1 /\ 0 <= j /\ j <= len - 1
@@ -173,41 +172,6 @@ let rec carry_wide_ tmp =
   lemma_carry_wide_spec_0 (as_seq h0 tmp);
   C.Loops.for 0ul FStar.UInt32.(clen -^ 1ul) inv f'
 
-
-(* [@"c_inline"] *)
-(* val carry_limb_: *)
-(*   t:felem -> *)
-(*   ctr:U32.t{U32.v ctr < len} -> *)
-(*   Stack unit *)
-(*     (requires (fun h -> live h t /\ carry_limb_pre (as_seq h t) (U32.v ctr))) *)
-(*     (ensures (fun h0 _ h1 -> live h0 t /\ live h1 t /\ modifies_1 t h0 h1 *)
-(*       /\ carry_limb_pre (as_seq h0 t) (U32.v ctr) *)
-(*       /\ as_seq h1 t == carry_limb_spec (as_seq h0 t) (U32.v ctr))) *)
-(* [@"c_inline"] *)
-(* let rec carry_limb_ tmp ctr = *)
-(*   if U32.(ctr =^ clen -^ 1ul) then () *)
-(*   else ( *)
-(*     let tctr = tmp.(ctr) in *)
-(*     let tctrp1 = tmp.(U32.(ctr+^1ul)) in *)
-(*     assert_norm(pow2 0 = 1); *)
-(*     Math.Lemmas.pow2_lt_compat limb_size 0; *)
-(*     Math.Lemmas.pow2_lt_compat limb_n limb_size; *)
-(*     Math.Lemmas.modulo_lemma (pow2 limb_size) (pow2 limb_n); *)
-(*     let r0 = (tctr) &^ ((limb_one <<^ climb_size) -^ limb_one) in *)
-(*     UInt.logand_mask #limb_n (v ( tctr)) limb_size; *)
-(*     Math.Lemmas.pow2_plus (limb_n - limb_size) (limb_size); *)
-(*     Math.Lemmas.modulo_modulo_lemma (v tctr) (pow2 limb_size) (pow2 (limb_n - limb_size)); *)
-(*     assert(v r0 = v tctr % pow2 limb_size); *)
-(*     assert(v r0 < pow2 limb_size); *)
-(*     let open Hacl.Bignum.Limb in *)
-(*     let c  = tctr >>^ climb_size in *)
-(*     Math.Lemmas.pow2_double_sum (limb_n - 1); *)
-(*     Math.Lemmas.lemma_div_lt (v tctr) (limb_n) (limb_size); *)
-(*     Math.Lemmas.pow2_le_compat (limb_n - 1) (limb_n - limb_size); *)
-(*     tmp.(ctr) <-  r0; *)
-(*     tmp.(U32.(ctr +^ 1ul)) <- tctrp1 +^ c; *)
-(*     carry_limb_ tmp (U32.(ctr +^ 1ul)) *)
-(*   ) *)
 
 #reset-options "--z3rlimit 100 --initial_fuel 1 --max_fuel 1"
 
